arm/Asmgenproof.v
@@ -23,13 +23,13 @@ Local Transparent Archi.ptr64.
 Definition match_prog (p: Mach.program) (tp: Asm.program) :=
   match_program (fun _ f tf => transf_fundef f = OK tf) eq p tp.
 
-Instance comp_transf_fundef: has_comp_transl_partial transf_fundef.
+Instance comp_transf_function: has_comp_transl_partial transf_function.
 Proof.
-  unfold transf_fundef, transf_function, transl_function.
-  intros [f|ef] ? H; monadInv H; trivial.
+  unfold transf_function, transl_function.
+  intros f ? H.
   destruct transl_code; simpl in *; try easy.
   destruct zlt; try easy.
-  now inv EQ.
+  now inv H.
 Qed.
 
 Lemma transf_program_match:
