backend/Debugvarproof.v
@@ -23,11 +23,11 @@ Require Import Debugvar.
 Definition match_prog (p tp: program) :=
   match_program (fun _ f tf => transf_fundef f = OK tf) eq p tp.
 
-Instance comp_transf_fundef: has_comp_transl_partial transf_fundef.
+Instance comp_transf_function: has_comp_transl_partial transf_function.
 Proof.
-  unfold transf_fundef, transf_function.
-  intros [f|ef] ? H; monadInv H; trivial.
-  now destruct ana_function; inv EQ.
+  unfold transf_function.
+  intros f ? H.
+  now destruct ana_function; inv H.
 Qed.
 
 Lemma transf_program_match:
